before final (lean)

final/lean/program/Final/arith.lean
@@ -3,7 +3,7 @@ example : Binop := Binop.Add
 
 
 inductive Expr
-| Num : ℕ → Expr
+| Num : Nat → Expr
 | Binop : Binop → Expr → Expr → Expr
 
 example : Expr := Expr.Num 1
@@ -11,13 +11,14 @@ example : Expr := Expr.Binop Binop.Add (Expr.Num 1) (Expr.Num 2)
 
 
 inductive val : Expr → Prop
-| DNat (n : ℕ) : val (Expr.Num n)
+| DNat (n : Nat) : val (Expr.Num n)
 
 example : val (Expr.Num 2) := val.DNat 2
 
 
-def apply_binop (op : Binop) (nl nr : ℕ) : ℕ :=
-  Binop.cases_on op (nl + nr) (nl - nr) (nl * nr) (nl / nr)
+def apply_binop (op : Binop) (nl nr : Nat) : Nat :=
+    Binop.casesOn op (nl + nr) (nl - nr) (nl * nr) (nl / nr)
+
 
 inductive steps : Expr → Expr → Prop
 | DLeft (op : Binop) (el el' er : Expr) :
@@ -30,12 +31,12 @@ inductive steps : Expr → Expr → Prop
   steps
     (Expr.Binop op el er)
     (Expr.Binop op el er')
-| DOp (op: Binop) (nl nr : ℕ) :
+| DOp (op: Binop) (nl nr : Nat) :
   steps
     (Expr.Binop op (Expr.Num nl) (Expr.Num nr))
     (Expr.Num (apply_binop op nl nr))
 
-notation e `↦`:35 e' := steps e e'
+notation:35 e " ↦ " e' => steps e e'
 
 example : (Expr.Binop Binop.Add (Expr.Num 1) (Expr.Num 2)) ↦ (Expr.Num 3) :=
    steps.DOp Binop.Add 1 2
