final/lean/program/Final/evals.lean
@@ -1,11 +1,11 @@
-import .arith
+import Final.arith
 
 inductive evals : Expr → Expr → Prop
 | Val (e : Expr) : evals e e
 | Step (e e_step e_val: Expr) :
   (e ↦ e_step) → evals e_step e_val → evals e e_val
 
-notation e `↦*`:35 e' := evals e e'
+notation:35 e " ↦* " e' => evals e e'
 
 example : (Expr.Binop Binop.Add (Expr.Num 1) (Expr.Num 2)) ↦* (Expr.Num 3) :=
   evals.Step
@@ -24,10 +24,10 @@ example : (Expr.Binop Binop.Add (Expr.Num 1) (Expr.Num 2)) ↦* (Expr.Num 3) :=
   end
 
 @[refl]
-lemma evals_refl (e : Expr) : e ↦* e := evals.Val e
+theorem evals_refl (e : Expr) : e ↦* e := evals.Val e
 
 @[trans]
-lemma evals_trans (e1 e2 e3 : Expr) (h1 : e1 ↦* e2) (h2 : e2 ↦* e3)
+theorem evals_trans (e1 e2 e3 : Expr) (h1 : e1 ↦* e2) (h2 : e2 ↦* e3)
   : e1 ↦* e3 :=
   begin
     induction h1,
@@ -40,13 +40,13 @@ lemma evals_trans (e1 e2 e3 : Expr) (h1 : e1 ↦* e2) (h2 : e2 ↦* e3)
     }
   end
 
-lemma transitive_left (b : Binop) (el el' er : Expr) :
+theorem transitive_left (b : Binop) (el el' er : Expr) :
   (el ↦* el') → (Expr.Binop b el er ↦* Expr.Binop b el' er) :=
   begin
     sorry -- Remove this line and add your proof
   end
 
-lemma transitive_right (b : Binop) (el er er' : Expr) :
+theorem transitive_right (b : Binop) (el er er' : Expr) :
   val el → (er ↦* er') → (Expr.Binop b el er ↦* Expr.Binop b el er') :=
   begin
     sorry -- Remove this line and add your proof
