final/lean/program/Final/f18.lean
@@ -1,0 +1,98 @@
+-- Some proofs from previous year's final
+
+section part1
+  variable (p q r s : Prop)
+    theorem and_commutativity (h: p ∧ q) : q ∧ p :=
+        ⟨ h.right, h.left ⟩
+
+    theorem demorgans_law : ¬(p ∨ q) ↔ ¬p ∧ ¬q :=
+    ⟨
+        fun h: ¬(p ∨ q) =>
+            have hnp: ¬p := fun hp: p =>
+                show False from h (Or.inl hp);
+            have hnq: ¬q := fun hq: q =>
+                show False from h (Or.inr hq);
+            show ¬p ∧ ¬q from ⟨ hnp, hnq ⟩,
+        fun h: ¬p ∧ ¬q =>
+            fun nr: p ∨ q =>
+                Or.elim nr (fun hp: p => h.left hp) (fun hq: q => h.right hq)
+    ⟩
+
+    theorem contraposition : (p → q) → (¬q → ¬p) :=
+        fun himp: p → q =>
+            fun hnp: ¬q =>
+                fun hp: p =>
+                    show False from hnp (himp hp)
+end part1
+
+section part2
+    variable (α : Type) (p q : α → Prop) (r : Prop)
+
+    theorem and_forall_dist : (∀ x, p x ∧ q x) ↔ (∀ x, p x) ∧ (∀ x, q x) :=
+    ⟨
+        fun h: ∀ x, p x ∧ q x =>
+            ⟨fun y => show p y from (h y).left,
+            fun y => show q y from (h y).right⟩,
+        fun h: (∀ x, p x) ∧ (∀ x, q x) =>
+            fun y => show p y ∧ q y from ⟨h.left y, h.right y⟩
+    ⟩
+
+    -- I can't prove unbound_prop without `em` from classical logic.
+    open Classical
+
+    theorem unbound_prop : (∀ x, p x ∨ r) ↔ (∀ x, p x) ∨ r :=
+    ⟨
+        fun h: ∀ x, p x ∨ r =>
+            (em r).elim
+                (fun hr: r =>
+                    show (∀ x, p x) ∨ r from Or.inr hr)
+                (fun hnr: ¬ r =>
+                    show (∀ x, p x) ∨ r from
+                        Or.inl fun y => (h y).resolve_right hnr),
+        fun h: (∀ x, p x) ∨ r =>
+            h.elim
+                (fun hl: ∀ x, p x =>
+                    fun y => Or.inl (hl y))
+                (fun hr: r =>
+                    fun _ => Or.inr (hr))
+    ⟩
+
+    variable (men : Type) (barber : men) (shaves : men → men → Prop)
+
+    theorem contradicts {p: Prop} : ¬(p ↔ (¬ p)) :=
+        fun h: p ↔ (¬ p) =>
+            have hnp: ¬ p := fun hp: p => (h.mp hp) hp;
+            have hp: p := h.mpr hnp;
+        show False from hnp hp
+
+    theorem barber_paradox : ¬ (∀ x : men, shaves barber x ↔ ¬ shaves x x) :=
+        fun h: ∀ x : men, shaves barber x ↔ ¬ shaves x x =>
+            show False from contradicts (h barber)
+end part2
+
+section part4
+    open Classical
+
+    variable (α : Type) (p q : α → Prop) (a : α) (r : Prop)
+
+    theorem dne {p : Prop} (h : ¬¬p) : p :=
+        Or.elim (em p)
+            (fun hp : p => hp)
+            (fun hnp : ¬p => absurd hnp h)
+
+    theorem forall_inverse : (∀ x, p x) ↔ ¬(∃ x, ¬p x) :=
+    ⟨
+        fun h: ∀ x, p x => byContradiction
+            (fun h1: ¬¬(∃ x, ¬p x) =>
+                Exists.elim (dne h1)
+                (fun w =>
+                    fun hw: ¬p w =>
+                        show False from hw (h w))),
+        fun h: ¬(∃ x, ¬p x) =>
+            fun x => byContradiction
+                (fun h1: ¬p x =>
+                    show False from h ⟨ x, h1 ⟩)
+
+    ⟩
+
+end part4
