final/lean/program/Final/inversion.lean
@@ -1,0 +1,5 @@
+import Final.arith
+
+@[simp]
+theorem val_inversion : ∀ e : Expr, val e → ∃ n : Nat, e = Expr.Num n :=
+  sorry -- Remove this line and add your proof
